ulib/experimental/Steel.PCMReference.fsti
@@ -1,0 +1,114 @@
+(*
+   Copyright 2020 Microsoft Research
+
+   Licensed under the Apache License, Version 2.0 (the "License");
+   you may not use this file except in compliance with the License.
+   You may obtain a copy of the License at
+
+       http://www.apache.org/licenses/LICENSE-2.0
+
+   Unless required by applicable law or agreed to in writing, software
+   distributed under the License is distributed on an "AS IS" BASIS,
+   WITHOUT WARRANTIES OR CONDITIONS OF ANY KIND, either express or implied.
+   See the License for the specific language governing permissions and
+   limitations under the License.
+*)
+
+module Steel.PCMReference
+
+open FStar.PCM
+open FStar.Ghost
+
+open Steel.Memory
+open Steel.Effect.Atomic
+open Steel.Effect
+
+#set-options "--ide_id_info_off"
+
+val read (#a:Type)
+         (#pcm:pcm a)
+         (r:ref a pcm)
+         (v0:erased a)
+  : SteelT (v:a { compatible pcm v0 v })
+           (pts_to r v0)
+           (fun _ -> pts_to r v0)
+
+val write (#a:Type)
+          (#pcm:pcm a)
+          (r:ref a pcm)
+          (v0:erased a)
+          (v1:a{frame_preserving pcm v0 v1 /\ pcm.refine v1})
+  : SteelT unit
+           (pts_to r v0)
+           (fun _ -> pts_to r v1)
+
+val alloc (#a:Type)
+          (#pcm:pcm a)
+          (x:a{compatible pcm x x /\ pcm.refine x })
+  : SteelT (ref a pcm)
+           emp
+           (fun r -> pts_to r x)
+
+val free (#a:Type)
+         (#p:pcm a)
+         (r:ref a p)
+         (x:erased a{exclusive p x /\ p.refine p.p.one})
+  : SteelT unit (pts_to r x) (fun _ -> pts_to r p.p.one)
+
+val split (#a:Type)
+          (#p:pcm a)
+          (r:ref a p)
+          (v:erased a)
+          (v0:erased a)
+          (v1:erased a)
+  : Steel unit (pts_to r v)
+               (fun _ -> pts_to r v0 `star` pts_to r v1)
+               (requires fun _ ->
+                 composable p v0 v1 /\
+                 v == hide (op p v0 v1))
+               (ensures fun _ _ _ -> True)
+
+val gather (#a:Type)
+           (#p:FStar.PCM.pcm a)
+           (r:ref a p)
+           (v0:erased a)
+           (v1:erased a)
+  : SteelT (_:unit{composable p v0 v1})
+           (pts_to r v0 `star` pts_to r v1)
+           (fun _ -> pts_to r (op p v0 v1))
+
+let fact_valid_compat (#a:Type) (#pcm:pcm a)
+                      (fact:stable_property pcm)
+                      (v:erased a)
+  = squash (forall z. compatible pcm v z ==> fact z)
+
+val witness (#a:Type) (#pcm:pcm a)
+            (r:ref a pcm)
+            (fact:stable_property pcm)
+            (v:erased a)
+            (_:fact_valid_compat fact v)
+  : SteelT unit (pts_to r v)
+                (fun _ -> pts_to r v `star` pure (witnessed r fact))
+
+val recall (#a:Type u#1) (#pcm:pcm a) (#fact:property a)
+           (r:ref a pcm)
+           (v:erased a)
+  : SteelT (v1:erased a{compatible pcm v v1})
+           (pts_to r v `star` pure (witnessed r fact))
+           (fun v1 -> pts_to r v `star` pure (fact v1))
+
+val select_refine (#a:Type u#1) (#p:pcm a)
+                  (r:ref a p)
+                  (x:erased a)
+                  (f:(v:a{compatible p x v}
+                      -> GTot (y:a{compatible p y v /\
+                                  frame_compatible p x v y})))
+   : SteelT  (v:a{compatible p x v /\ p.refine v})
+             (pts_to r x)
+             (fun v -> pts_to r (f v))
+
+val upd_gen (#a:Type) (#p:pcm a) (r:ref a p) (x y:erased a)
+            (f:frame_preserving_upd p x y)
+  : SteelT unit
+           (pts_to r x)
+           (fun _ -> pts_to r y)
